Cleanup in SpecViaZ
 Note that in NSig (and hence NMake and BigN), to_N is now
 Z.to_N (to_Z ...) instead of Z.abs_N (to_Z ...). This doesn't
 change the result (since to_Z create non-negative integers),
 but some proofs may have to be adapted

git-svn-id: svn+ssh://scm.gforge.inria.fr/svn/coq/trunk@14250 85f007b7-540e-0410-9357-904b9bb8a0f7

theories/Numbers/Natural/BigN/NMake.v
@@ -69,7 +69,7 @@ Module Make (W0:CyclicType) <: NType.
  apply Zpower_le_monotone2; auto with zarith.
  Qed.
 
- Definition to_N (x : t) := Zabs_N (to_Z x).
+ Definition to_N (x : t) := Z.to_N (to_Z x).
 
  (** * Zero, One *)
 
@@ -817,7 +817,7 @@ Module Make (W0:CyclicType) <: NType.
  Theorem spec_pow : forall x y, [pow x y] = [x] ^ [y].
  Proof.
  intros. unfold pow, to_N.
- now rewrite spec_pow_N, Z_of_N_abs, Zabs_eq by apply spec_pos.
+ now rewrite spec_pow_N, Z2N.id by apply spec_pos.
  Qed.
 
 
