theories/Numbers/Integer/SpecViaZ/ZSig.v
@@ -91,7 +91,7 @@ Module Type ZType.
  Parameter spec_mul: forall x y, [mul x y] = [x] * [y].
  Parameter spec_square: forall x, [square x] = [x] *  [x].
  Parameter spec_pow_pos: forall x n, [pow_pos x n] = [x] ^ Zpos n.
- Parameter spec_pow_N: forall x n, [pow_N x n] = [x] ^ Z_of_N n.
+ Parameter spec_pow_N: forall x n, [pow_N x n] = [x] ^ Z.of_N n.
  Parameter spec_pow: forall x n, [pow x n] = [x] ^ [n].
  Parameter spec_sqrt: forall x, [sqrt x] = Z.sqrt [x].
  Parameter spec_log2: forall x, [log2 x] = Z.log2 [x].
